semantics for non-deterministic monoid
in ll_semnd.v, converted from ll_sem.v
note different proofs of tens_assocr_lem and uncurry_sem
started on completeness

ll/ll_comp.v
@@ -6,7 +6,7 @@ Set Implicit Arguments.
 Add LoadPath "../general".
 Add LoadPath "../modal".
 Require Import gen genT ddT swappedT.
-Require Import fmlsext lldefs ll_exch ll_camq ll_sem.
+Require Import fmlsext lldefs ll_exch ll_camq ll_semnd.
 
 From Coq Require Import ssreflect.
 
@@ -15,8 +15,8 @@ From Coq Require Import ssreflect.
 Definition FLM {V} := list (LLfml V).
 (* m is app, e is [] *)
 (*
-Print Implicit comm_monoid.
-Print Implicit app.
+Print Implicit comm_monoid_nd.
+Print Implicit merge.
 Print Implicit nil.
 Print Implicit tens_sem.
 Print tens_sem.
@@ -27,10 +27,28 @@ Print Implicit sem.
 Print Implicit fact.
 *)
 
+Definition mergeP {T} X Y Z := inhabited (@merge T X Y Z).
+
 (* problem, lists do not form a comm_monoid,
   need to use equivalence classes - at deductive or semantic level? 
-Lemma comm_monoid_list X : comm_monoid (@app X) [].
-*)
+  or use non-deterministic monoid, as in ll_semnd.v *)
+Lemma comm_monoid_nd_list X : comm_monoid_nd (@mergeP X) [].
+Proof. unfold comm_monoid_nd. 
+repeat apply conj ; intros ; apply conj ;
+try (apply inhabited_ind ; intro ; apply inhabits).
+- intro m. destruct m.  destruct H.  destruct H0.
+destruct (merge_assoc X1 X0). 
+exact (merge3RI _ _ _ _ _ _ (inhabits m0) (inhabits m)).
+- intro m. destruct m.  destruct H.  destruct H0.
+destruct (merge_assoc (merge_sym X1) (merge_sym X0)). 
+exact (merge3LI _ _ _ _ _ _ (inhabits (merge_sym m0)) (inhabits (merge_sym m))).
+- exact (merge_sym X0).
+- exact (merge_sym X0).
+- apply inhabited_ind. apply merge_RnilE. 
+- intro. subst. apply inhabits. apply merge_Rnil.
+- apply inhabited_ind. apply merge_LnilE. 
+- intro. subst. apply inhabits. apply merge_Lnil. Qed.
+
 
 (* the Girard paper defines the set of members of the monoid 
   corresponding to a formula in terms of provability, which makes
@@ -43,7 +61,47 @@ Lemma comm_monoid_list X : comm_monoid (@app X) [].
 Definition pr_sem V A G := inhabited (derrec (@maell_rules V) emptyT (A :: G)).
 Definition pr_seml V As G := 
   inhabited (derrec (@maell_rules V) emptyT (As ++ G)).
+Definition pr_sv {V} v G := 
+  inhabited (derrec maell_rules emptyT (@Var V v :: G)).
 Definition prb {V} G := inhabited (derrec (@maell_rules V) emptyT G).
+
+Print Implicit sem.
+Print Implicit pr_sv.
+Print Implicit pr_sem.
+
+(* a condition of semantics generally (forall v : V, fact m bot (sv v)) *)
+(*
+note lemmas from ll_semnd.v
+Lemma dual_sem_1 : forall u, iff (dual_sem (eq e) u) (bot u).
+Lemma dual_sem_bot : dual_sem bot e.
+Lemma fact_bot : fact bot.
+Check dual_sem_1.
+Check dual_sem_bot.
+Check fact_bot.
+*)
+
+Lemma pr_sv_sem V v : @pr_sv V v = @pr_sem V (Var v).
+Proof. reflexivity. Qed.
+
+(* do we need this result? note, fact_pr_sem follows easily from it
+Lemma fact_pr_seml V As : fact mergeP prb (@pr_seml V As).
+Proof. unfold fact.  unfold dual_sem.  unfold lolli_sem.    intros.
+specialize (H As).  apply H.
+2: apply inhabits. 2: apply merge_simple_appr.
+intros.  destruct H0.  destruct H1.  apply inhabits.
+(* need result here, two different merges is transitive closure of swapped *)
+*)
+
+Lemma fact_pr_sem V A : fact mergeP prb (@pr_sem V A).
+Proof. unfold fact.  unfold dual_sem.  unfold lolli_sem.    intros.
+specialize (H [A]).  apply H.
+2: apply inhabits. 2: apply merge_simple_appr.
+intros.  destruct H0.  destruct H1.  apply inhabits.
+apply merge_singleL in H0.  cD.  subst.  apply (exch_maell X).
+swap_tac_Rc. Qed.
+
+Lemma fact_pr_sv V v : fact mergeP prb (@pr_sv V v).
+Proof. apply fact_pr_sem. Qed.
 
 (*
 Lemma pr_sem_tens V A B G : 
@@ -51,30 +109,53 @@ Lemma pr_sem_tens V A B G :
 Proof. unfold tens_sem. unfold pr_sem.
 *)
 
-(*
-Lemma fact_cs V A : fact (@app _) prb (@pr_sem V A).
-*)
-
 Lemma pr_sem_dual V A G : 
-  dual_sem (@app _) prb (pr_sem A) G -> pr_sem (@dual V A) G.
+  dual_sem mergeP prb (pr_sem A) G -> pr_sem (@dual V A) G.
 Proof. unfold dual_sem. unfold lolli_sem.  unfold pr_sem.
 intros lav. specialize (lav [dual A]).  unfold prb in lav.
-require lav. apply inhabits. apply maell_id.
-destruct lav.  apply inhabits.
-apply (exch_maell X). swap_tac_Rc. Qed.
+apply lav.  apply inhabits. apply maell_id.
+apply inhabits. apply merge_simple_appr. Qed.
 
-(* this one requires cut rule *)
+(* this one requires cut rule
 Lemma dual_pr_sem V A G : 
-  pr_sem (@dual V A) G -> dual_sem (@app _) prb (pr_sem A) G.
+  pr_sem (@dual V A) G -> dual_sem mergeP prb (pr_sem A) G.
 Proof. unfold dual_sem. unfold lolli_sem.  unfold pr_sem.
-intros idag v iav. unfold prb.
-destruct idag.  destruct iav.  apply inhabits.
-destruct (fst (cut_adm_maell_Q A X0 X)).
-eapply (d _ _ _ eq_refl eq_refl). apply merge_simple_appr. Qed.
+intros idag v w iav mgvw. unfold prb.
+destruct idag.  destruct iav.  destruct mgvw.  apply inhabits.
+destruct (fst (cut_adm_maell_Q A X0 X)). Qed.
+*)
+
+Print Implicit dual_sem_1_eq.
+
+(* now we need to show that the semantics defined using pr_sv
+  corresponds to pr_sem (at least, for completeness, one way) *)
+(*
+Lemma sem_pr V A X : sem mergeP [] prb pr_sv A X -> @pr_sem V A X.
+Proof. induction A ; simpl.
+- unfold pr_sv. unfold pr_sem. tauto.
+- unfold dual_sem. unfold pr_sem. unfold lolli_sem.
+unfold pr_sv. unfold prb. intro.
+specialize (H [DVar v]). apply H.
+2: apply inhabits. 2: apply merge_simple_appr.
+apply inhabits. pose (maell_id (Var v)).  simpl in d. exact d.
+- unfold prb. unfold pr_sem. apply inhabited_ind. intro. apply inhabits.
+eapply derI.  eapply princ_maellI. eapply (OSgctxt_eq _ _ _ []).
+apply Bot_p.  eapply Botrule_I. reflexivity. reflexivity.
+apply dersrec_singleI. exact X0.
+- unfold pr_sem. intro. apply inhabits.
+eapply derI.  eapply princ_maellI. eapply (OSgctxt_eq _ _ _ []).
+apply Top_p.  eapply Toprule_I. reflexivity. reflexivity. apply dlNil.
+- rewrite (dual_sem_1_eq (@prb V) (comm_monoid_nd_list _)).
+unfold pr_sem. unfold dual_sem. unfold lolli_sem.
+intro pmb. specialize (pmb [One V] (One V :: X)).
+unfold prb in pmb. apply pmb.
+2: apply inhabits. 2: apply merge_simple_appr.
+apply inhabits. eapply derI. apply one_maellI. apply Onerule_I. apply dlNil.
+- intro dde. unfold dual_sem in dde. unfold lolli_sem in dde.
+unfold pr_sem. unfold prb in dde. apply (dde [Zero V]).
+2: apply inhabits. 2: apply merge_simple_appr. tauto.
+- TBC
+*)
 
 
-
-
-
-  
 
